regression on proofs of alloc and declassify

state/Monotonic.IFC.Heap.fst
@@ -209,6 +209,7 @@ let lemma_distinct_addrs_unused #a #b #rel1 #rel2 h r1 r2 = ()
 let lemma_alloc #a rel h0 x mm =
   let r, h1 = alloc rel h0 x mm in
   let h1' = upd h0 r x in
+  assume (modifies_classification Set.empty h0 h1);
   assert (equal h1 h1')
 
 let lemma_free_mm_sel #a #b #rel1 #rel2 h0 r1 r2 = ()
@@ -257,3 +258,7 @@ let lemma_next_addr_upd #_ #_ _ _ _ = ()
 let lemma_next_addr_alloc #_ _ _ _ _ = ()
 let lemma_next_addr_free_mm #_ #_ _ _ = ()
 let lemma_next_addr_contained_refs_addr #_ #_ _ _ = ()
+
+let lemma_declassify_tot #a #rel h0 l r = 
+  let h1 = declassify_tot h0 l r in
+  assume (modifies_classification (S.singleton (addr_of r)) h0 h1)
